complete Imp chapter

Imp.v
@@ -2523,8 +2523,131 @@ End BreakImp.
     about making up a concrete Notation for [for] loops, but feel free
     to play with this too if you like.) *)
 
-(* FILL IN HERE
+(* 1h20min - way too boring *)
 
-    [] *)
+Print com.
+Module ForImp.
+
+Inductive com : Type :=
+  | CSkip
+  | CAsgn (x : string) (a : aexp)
+  | CSeq (c1 c2 : com)
+  | CIf (b : bexp) (c1 c2 : com)
+  | CWhile (b : bexp) (c : com)
+  | CFor (cinit : com) (b : bexp) (cupdate c : com).
+
+Notation "'skip'"  :=
+         CSkip (in custom com at level 0) : com_scope.
+Notation "x := y"  :=
+         (CAsgn x y)
+            (in custom com at level 0, x constr at level 0,
+             y at level 85, no associativity) : com_scope.
+Notation "x ; y" :=
+         (CSeq x y)
+           (in custom com at level 90, right associativity) : com_scope.
+Notation "'if' x 'then' y 'else' z 'end'" :=
+         (CIf x y z)
+           (in custom com at level 89, x at level 99,
+            y at level 99, z at level 99) : com_scope.
+Notation "'while' x 'do' y 'end'" :=
+         (CWhile x y)
+            (in custom com at level 89, x at level 99, y at level 99) : com_scope.
+Notation "'for' w ; x ; y 'do' z 'end'" :=
+         (CFor w x y z)
+            (in custom com at level 89,
+                w at level 88, x at level 88, 
+                y at level 88, z at level 88) : com_scope.
+
+Inductive ceval : com -> state -> state -> Prop :=
+  | E_Skip : forall st,
+      st =[ skip ]=> st
+  | E_Asgn  : forall st a n x,
+      aeval st a = n ->
+      st =[ x := a ]=> (x !-> n ; st)
+  | E_Seq : forall c1 c2 st st' st'',
+      st  =[ c1 ]=> st'  ->
+      st' =[ c2 ]=> st'' ->
+      st  =[ c1 ; c2 ]=> st''
+  | E_IfTrue : forall st st' b c1 c2,
+      beval st b = true ->
+      st =[ c1 ]=> st' ->
+      st =[ if b then c1 else c2 end]=> st'
+  | E_IfFalse : forall st st' b c1 c2,
+      beval st b = false ->
+      st =[ c2 ]=> st' ->
+      st =[ if b then c1 else c2 end]=> st'
+  | E_WhileFalse : forall b st c,
+      beval st b = false ->
+      st =[ while b do c end ]=> st
+  | E_WhileTrue : forall st st' st'' b c,
+      beval st b = true ->
+      st  =[ c ]=> st' ->
+      st' =[ while b do c end ]=> st'' ->
+      st  =[ while b do c end ]=> st''
+  | E_For : forall b st st' ci cu c,
+      st =[ ci ; while b do c ; cu end ]=> st' ->
+      st =[ for ci ; b ; cu do c end ]=> st'
+  where "st '=[' c ']=>' st'" := (ceval c st st').
+
+Example for_example1 :
+  ( X !-> 0 ) =[
+    for Y := 0 ; Y <= 1 ; Y := Y + 1 do
+      X := X + 2
+    end
+  ]=> ( Y !-> 2 ; X !-> 4 ; Y !-> 1 ; X !-> 2 ; Y !-> 0 ; X !-> 0 ).
+Proof.
+  constructor.
+  Definition st0 := ( Y !-> 0 ; X !-> 0 ). 
+  apply E_Seq with st0.
+  { apply E_Asgn. reflexivity. }
+  { apply E_WhileTrue with ( Y !-> 1 ; X !-> 2 ; st0 ).
+    { reflexivity. }
+    { apply E_Seq with ( X !-> 2 ; st0 );
+        apply E_Asgn; reflexivity. }
+    { Definition st1 := ( Y !-> 1 ; X !-> 2 ; st0 ). 
+      apply E_WhileTrue with ( Y !-> 2; X !-> 4; st1 ).
+      { reflexivity. }
+      { apply E_Seq with ( X !-> 4 ; st1 );
+        apply E_Asgn; reflexivity. }
+      { apply E_WhileFalse. reflexivity. }
+    }
+  }
+Qed.
+
+Theorem ceval_deterministic: forall c st st1 st2,
+     st =[ c ]=> st1  ->
+     st =[ c ]=> st2 ->
+     st1 = st2.
+Proof.
+  intros c st st1 st2 E1 E2.
+  generalize dependent st2.
+  induction E1; intros st2 E2; inversion E2; subst.
+  - (* E_Skip *) reflexivity.
+  - (* E_Asgn *) reflexivity.
+  - (* E_Seq *)
+    rewrite (IHE1_1 st'0 H1) in *.
+    apply IHE1_2. assumption.
+  - (* E_IfTrue, b evaluates to true *)
+      apply IHE1. assumption.
+  - (* E_IfTrue,  b evaluates to false (contradiction) *)
+      rewrite H in H5. discriminate.
+  - (* E_IfFalse, b evaluates to true (contradiction) *)
+      rewrite H in H5. discriminate.
+  - (* E_IfFalse, b evaluates to false *)
+      apply IHE1. assumption.
+  - (* E_WhileFalse, b evaluates to false *)
+    reflexivity.
+  - (* E_WhileFalse, b evaluates to true (contradiction) *)
+    rewrite H in H2. discriminate.
+  - (* E_WhileTrue, b evaluates to false (contradiction) *)
+    rewrite H in H4. discriminate.
+  - (* E_WhileTrue, b evaluates to true *)
+    rewrite (IHE1_1 st'0 H3) in *.
+    apply IHE1_2. assumption.
+  - rewrite (IHE1 st2 H5). reflexivity.
+Qed.
+
+End ForImp.
+(** [] *)
 
 (* 2024-01-03 15:00 *)
